src/ProbabilisticProgramming/RandomSource.dfy
@@ -18,10 +18,54 @@ module Rand {
 
   ghost const prob: iset<Bitstream> -> real
 
+  // Equation (2.37)
+  function Head(s: Bitstream): bool {
+    s(0)
+  }
+
+  // Equation (2.38)
+  function Tail(s: Bitstream): (s': Bitstream) {
+    (n: nat) => s(n+1)
+  }
+
+  function IterateTail(s: Bitstream, n: nat): (t: Bitstream)
+    ensures t(0) == s(n)
+  {
+    if n == 0 then s else IterateTail(Tail(s), n - 1)
+  }
+
+  lemma TailOfIterateTail(s: Bitstream, n: nat)
+    ensures Tail(IterateTail(s, n)) == IterateTail(s, n + 1)
+  {}
+
+  // Equation (2.41)
+  function Drop(n: nat, s: Bitstream): (s': Bitstream)
+    ensures Head(s') == s(n)
+  {
+    if n == 0 then s else Drop(n - 1, Tail(s))
+  }
+
   /*******
    Lemmas
   *******/
 
   lemma {:axiom} ProbIsProbabilityMeasure()
     ensures Measures.IsProbability(eventSpace, sampleSpace, prob)
+
+  // Equation (2.68) && (2.77)
+  lemma {:axiom} CoinHasProbOneHalf(b: bool)
+    ensures
+      var e := (iset s | Head(s) == b);
+      && e in eventSpace
+      && prob(e) == 0.5
+
+  // Equation (2.82)
+  lemma {:axiom} MeasureHeadDrop(n: nat, s: Bitstream)
+    ensures
+      && (iset s | Head(Drop(n, s))) in eventSpace
+      && prob(iset s | Head(Drop(n, s))) == 0.5
+
+  // Equation (2.78)
+  lemma {:axiom} TailIsMeasurePreserving()
+    ensures Measures.IsMeasurePreserving(eventSpace, prob, eventSpace, prob, Tail)
 }
